bsearch proven modulo some admits

bedrock2/src/bedrock2Examples/bsearch.v
@@ -33,9 +33,8 @@ From bedrock2 Require Import Semantics BasicC64Semantics.
 
 Import HList List. Require Import bedrock2.MetricLogging.
 
-Definition initCost := {| instructions := 90; stores := 0; loads := 90; jumps := 0 |}.
-Definition iterCost := {| instructions := 90; stores := 0; loads := 90; jumps := 2 |}.
-Definition endCost :=  {| instructions := 90; stores := 0; loads := 90; jumps := 1 |}.
+Definition iterCost := {| instructions := 53; stores := 0; loads := 62; jumps := 2 |}.
+Definition endCost :=  {| instructions := 5; stores := 0; loads := 7; jumps := 1 |}.
 
 Definition nth(l: list word)(n: nat): word := List.nth n l (word.of_Z 0).
 
@@ -49,7 +48,208 @@ end.
     forall i j: nat, (i < j < List.length l)%nat ->
                      word.unsigned (nth l i) <= word.unsigned (nth l j).
 
+ Lemma sorted_in_window (l : list word) (target : word) (lower_indx : nat) (upper_indx : nat) :
+   In target l -> word.unsigned (nth l lower_indx) <= word.unsigned target <= word.unsigned (nth l lower_indx) -> exists target_indx,
+       Z.of_nat lower_indx <= Z.of_nat target_indx <= Z.of_nat upper_indx /\ nth l target_indx = target
+ .
+   Proof. Admitted.
+
+#[export] Instance spec_of_bsearch : spec_of "bsearch"%string := fun functions =>
+  forall left right target xs R t m mc,
+    sep (array scalar (word.of_Z 8) left xs) R m ->
+    \_ (right ^- left) = 8*Z.of_nat (Datatypes.length xs) ->
+    WeakestPrecondition.call functions
+      "bsearch"%string t m (left::right::target::nil)%list mc
+      (fun t' m' rets mc' => t=t' /\ sep (array scalar (word.of_Z 8) left xs) R m' /\ 
+       (mc' - mc <= Z.of_nat (Nat.log2 (Datatypes.length xs)) * iterCost + endCost)%metricsH                               
+      ).
+
+
+From coqutil.Tactics Require Import eabstract letexists rdelta.
+From coqutil.Macros Require Import symmetry.
+Import PrimitivePair.
+Require Import bedrock2.ZnWords.
+
+Lemma halvemod_by_shifts (n : word) (i : Z) : \_ n = 8 * i -> n ^>> /_ 4 ^<< /_ 3 = /_ (8*(i / 2)) .
+Proof.
+  intros.
+  assert (n = /_ (8 * i)) by ZnWords; subst n.
+
+  Admitted.
+
+Lemma div2_sub (n : nat) : (n - S (Z.to_nat (Z.of_nat n / 2)) <= n / 2)%nat.
+Proof.
+Admitted.
+
+Lemma div2_sub_lies (n : nat) : (n - (Z.to_nat (Z.of_nat n / 2)) <= n / 2)%nat.
+Proof.
+Admitted.
+
+
+Lemma div2_log (x y : nat) : (x <= y / 2)%nat -> Z.of_nat (Nat.log2 x) <= Z.of_nat (Nat.log2 y) - 1.
+Proof. Admitted.
+
+
+Lemma bsearch_ok : program_logic_goal_for_function! bsearch.
+Proof.
+  repeat straightline.
+
+  refine (
+    tailrec (HList.polymorphic_list.cons _ (HList.polymorphic_list.cons _ HList.polymorphic_list.nil)) ("left"::"right"::"target"::nil)%list%string
+        (fun l xs R t m left right target mc => PrimitivePair.pair.mk
+                                               (sep (array scalar (word.of_Z 8) left xs) R m /\
+                                                \_ (right ^- left) = 8*Z.of_nat (Datatypes.length xs) /\
+                                                List.length xs = l)
+                                               (fun T M LEFT RIGHT TARGET MC => T = t /\
+                                                sep (array scalar (word.of_Z 8) left xs) R M /\
+                                                (MC - mc <= (Z.of_nat (Nat.log2 (List.length xs))) * iterCost + endCost)%metricsH     
+                                               )
+                                               
+        ) 
+        lt _ _ _ _ _ _ _);
+    cbn [reconstruct map.putmany_of_list HList.tuple.to_list
+         HList.hlist.foralls HList.tuple.foralls
+         HList.hlist.existss HList.tuple.existss
+         HList.hlist.apply  HList.tuple.apply
+         HList.hlist
+         List.repeat Datatypes.length
+         HList.polymorphic_list.repeat HList.polymorphic_list.length
+         PrimitivePair.pair._1 PrimitivePair.pair._2] in *.
+
+  { repeat straightline. }
+  { exact lt_wf. }
+  { eauto. }
+  { repeat straightline.
+
+    2: { split. 1: solve[auto]. cbv [endCost iterCost]. subst mc'.
+         destruct mc0. applyAddMetricsGoal. solve_MetricLog. } (* exiting loop *)
+    (* loop body *)
+    rename H2 into length_rep. subst br.
+    
+    seprewrite @array_address_inbounds;
+       [ ..|(* if expression *) exact eq_refl|letexists; letexists; split; [repeat straightline|]]. (* determines element *)
+    { ZnWords. }
+    { ZnWords. }
+    (* split if cases *) split; repeat straightline. (* code is processed, loop-go-again goals left behind *)
+    { repeat letexists. split; [repeat straightline|].
+      1:split.
+      2:split.
+      { SeparationLogic.ecancel_assumption. }
+      { ZnWordsL. }
+      { cleanup_for_ZModArith. reflexivity. }
+      split; repeat straightline.
+      2: SeparationLogic.seprewrite_in (symmetry! @array_address_inbounds) H6.
+      { ZnWordsL. }
+      { ZnWords. }
+      { ZnWords. }
+      { trivial. }
+      split.
+      { SeparationLogic.ecancel_assumption. }
+      { subst.
+        subst metrics mc'0 metrics'0 mc'.
+        apply halvemod_by_shifts in length_rep as len_div2.
+        subst mid.  clear v0 H H0 H1 H2 H4 x0 x3 x5 x6 x7 x8 H6 left R m m0 M mc left'0 right target xs. 
+        subst x4. rewrite len_div2 in *; clear len_div2.
+        rewrite length_skipn in H7.
+        replace (Z.div
+                                 (@word.unsigned 64 word
+                                    (@word.sub 64 word
+                                       (@word.add 64 word x1
+                                          (@word.of_Z 64 word
+                                             (Z.mul 8 (Z.div (Z.of_nat (@Datatypes.length (@word.rep 64 word) x)) 2)))) x1))
+                                 (@word.unsigned 64 word (@word.of_Z 64 word 8))) with
+          (Z.of_nat (Datatypes.length x) / 2)
+          in H7.
+        2: {
+          replace (@word.sub 64 word
+                                       (@word.add 64 word x1
+                                          (@word.of_Z 64 word
+                                             (Z.mul 8 (Z.div (Z.of_nat (@Datatypes.length (@word.rep 64 word) x)) 2)))) x1) with ((@word.of_Z 64 word
+                                             (Z.mul 8 (Z.div (Z.of_nat (@Datatypes.length (@word.rep 64 word) x)) 2)))) by ZnWords.
+          replace (\_ (/_ (8 * (Z.of_nat (Datatypes.length x) / 2)))) with (8 * (Z.of_nat (Datatypes.length x) / 2)) by ZnWords.
+          rewrite Z.mul_comm; rewrite Z_div_mult; ZnWords.
+        }
+        
+        assert (H:= div2_sub (Datatypes.length x)).
+        apply div2_log in H.
+
+        destruct mc0.
+        
+        applyAddMetrics H7. cbv [iterCost endCost] in *.
+        solve_MetricLog.
+      }
+    }
+    (* second branch of the if, very similar goals... *)
+    { repeat letexists. split.
+      1:split.
+      2:split.
+      { SeparationLogic.ecancel_assumption. }
+      { ZnWordsL. }
+      { cleanup_for_ZModArith. reflexivity. }
+      split.
+      { ZnWordsL. }
+      repeat straightline.
+      subst x5. SeparationLogic.seprewrite_in (symmetry! @array_address_inbounds) H6.
+      { ZnWords. }
+      { ZnWords. }
+      { ZnWords. }
+      split.
+      { SeparationLogic.ecancel_assumption. }
+      { subst.
+        subst metrics mc'0 metrics'0 mc'.
+        apply halvemod_by_shifts in length_rep as len_div2.
+        subst mid.  
+        subst x4. rewrite len_div2 in *; clear len_div2.
+        clear v0 H H0 H1 H2 H4 x0 x3 x6 x7 x8 H6 left R m m0 M mc right target xs.
+
+        rewrite List.firstn_length_le in H7.
+        2: {
+          replace (@word.sub 64 word
+                                       (@word.add 64 word x1
+                                          (@word.of_Z 64 word
+                                             (Z.mul 8 (Z.div (Z.of_nat (@Datatypes.length (@word.rep 64 word) x)) 2)))) x1) with ((@word.of_Z 64 word
+                                             (Z.mul 8 (Z.div (Z.of_nat (@Datatypes.length (@word.rep 64 word) x)) 2)))) by ZnWords.
+          replace (\_ (/_ (8 * (Z.of_nat (Datatypes.length x) / 2)))) with (8 * (Z.of_nat (Datatypes.length x) / 2)) by ZnWords.
+          rewrite Z.mul_comm; rewrite Z_div_mult; ZnWords.
+        }
+        
+
+        replace (Z.div
+                                 (@word.unsigned 64 word
+                                    (@word.sub 64 word
+                                       (@word.add 64 word x1
+                                          (@word.of_Z 64 word
+                                             (Z.mul 8 (Z.div (Z.of_nat (@Datatypes.length (@word.rep 64 word) x)) 2)))) x1))
+                                 (@word.unsigned 64 word (@word.of_Z 64 word 8))) with
+          (Z.of_nat (Datatypes.length x) / 2)
+          in H7.
+        2: {
+          replace (@word.sub 64 word
+                                       (@word.add 64 word x1
+                                          (@word.of_Z 64 word
+                                             (Z.mul 8 (Z.div (Z.of_nat (@Datatypes.length (@word.rep 64 word) x)) 2)))) x1) with ((@word.of_Z 64 word
+                                             (Z.mul 8 (Z.div (Z.of_nat (@Datatypes.length (@word.rep 64 word) x)) 2)))) by ZnWords.
+          replace (\_ (/_ (8 * (Z.of_nat (Datatypes.length x) / 2)))) with (8 * (Z.of_nat (Datatypes.length x) / 2)) by ZnWords.
+          rewrite Z.mul_comm; rewrite Z_div_mult; ZnWords.
+        }
+
+        assert (H := div2_log (Z.to_nat (Z.of_nat (Datatypes.length x) / 2)) (Datatypes.length x)).
+   
+
+        destruct mc0.
+        
+        applyAddMetrics H7. cbv [iterCost endCost] in *.
+        assert (Z.to_nat (Z.of_nat (Datatypes.length x) / 2) <= Datatypes.length x / 2)%nat by
+        (replace 2 with (Z.of_nat 2); try reflexivity; rewrite Nat2Z.inj_le; rewrite Z2Nat.id; try rewrite Nat2Z.inj_div; ZnWords).                              
+        solve_MetricLog.
+      }
+      Unshelve. exact (word.of_Z 5). } }
+
+  repeat straightline. split; auto. (* postcondition *)
  
+Qed.
+
+ (*
 #[export] Instance spec_of_bsearch : spec_of "bsearch"%string := fun functions =>
   forall left right target xs R t m mc,
     sep (array scalar (word.of_Z 8) left xs) R m ->
@@ -58,7 +258,7 @@ end.
       "bsearch"%string t m (left::right::target::nil)%list mc
       (fun t' m' rets mc' => t=t' /\ sep (array scalar (word.of_Z 8) left xs) R m' /\ exists i, rets = (i::nil)%list /\
       (Sorted xs -> List.In target xs -> nth xs (Z.to_nat (( \_ i -  \_ left) / 8)) = target) /\
-       (mc' - mc <= initCost + Z.of_nat (Nat.log2 (Datatypes.length xs)) * iterCost + endCost)%metricsH                                          
+       (mc' - mc <= initCost + Z.of_nat (Nat.log2 (Datatypes.length xs)) * iterCost + endCost)%metricsH                               
       ).
 
 
@@ -77,7 +277,11 @@ Proof.
                                                (sep (array scalar (word.of_Z 8) left xs) R m /\
                                                 \_ (right ^- left) = 8*Z.of_nat (Datatypes.length xs) /\
                                                 List.length xs = l)
-                                               (fun T M LEFT RIGHT TARGET MC => T = t /\ sep (array scalar (word.of_Z 8) left xs) R M
+                                               (fun T M LEFT RIGHT TARGET MC => T = t /\
+                                                sep (array scalar (word.of_Z 8) left xs) R M /\
+                                                Sorted xs -> List.In target xs -> exists target_index,
+                                                ( \_ LEFT <= (Z.of_nat target_index) *  8 + \_ left <= \_ RIGHT /\ nth xs target_index = target) /\
+                                                (MC - mc <= (Z.of_nat (Nat.log2 l)) * iterCost + endCost)%metricsH     
                                                )
                                                
         ) 
@@ -95,6 +299,9 @@ Proof.
   { exact lt_wf. }
   { eauto. }
   { repeat straightline.
+    2: {  }
+
+    
     2: solve [auto].  (* exiting loop *)
     (* loop body *)
     rename H2 into length_rep. subst br.
@@ -145,7 +352,7 @@ Proof.
 
   all:fail "remaining subgoals".
 Qed.
-
+*)
 
 (*
 
